# 分数乘法练习题(一)

$\dfrac{1}{2}×8=\qquad \dfrac{1}{3}×9= \qquad \dfrac{4}{9}×7=\\[1em]
\dfrac{9}{11}×8=\qquad \dfrac{3}{6}×\dfrac{2}{9}=\qquad \dfrac{5}{9}×\dfrac{7}{2}=\\[1em]
\dfrac{1}{10}×\dfrac{9}{4}=\qquad
\dfrac{23}{4}×\dfrac{2}{6}=\qquad
\dfrac{76}{5}×\dfrac{1}{38}=\\[1em]
\dfrac{87}{9}×\dfrac{3}{19}=\qquad
\dfrac{15}{4}×\dfrac{1}{3}=\qquad
\dfrac{56}{2}×\dfrac{1}{8}=\\[1em]
\dfrac{2}{9}×\dfrac{3}{18}=\qquad
\dfrac{1}{4}×3=\qquad
\dfrac{12}{13}×26=\\[1em]
\dfrac{19}{6}×\dfrac{3}{2}=\qquad
\dfrac{2}{3}×\dfrac{7}{2}=\qquad
\dfrac{6}{7}×\dfrac{14}{2}=\\[1em]
\dfrac{16}{7}×\dfrac{21}{4}=\qquad
\dfrac{29}{3}×6=\qquad
\dfrac{1}{2}×6=\\[1em]
\dfrac{1}{6}×9=\qquad
\dfrac{4}{3}×7=\qquad
\dfrac{9}{4}×8=\\[1em]
\dfrac{3}{12}×\dfrac{2}{9}=\qquad
\dfrac{5}{9}×\dfrac{7}{5} =\qquad
\dfrac{1}{10}×\dfrac{9}{2}=\\[2em]
\dfrac{24}{4}×\dfrac{2}{6}=\qquad
\dfrac{76}{7}×\dfrac{1}{38}=\qquad
\dfrac{87}{6}×\dfrac{3}{19}=\\[2em]
\dfrac{12}{4}×\dfrac{1}{3}=\qquad
\dfrac{56}{2}×\dfrac{1}{7}=\qquad
\dfrac{2}{9}×\dfrac{6}{18}=\\[2em]
\dfrac{1}{4}×7=\qquad
\dfrac{3}{13}×26=\qquad
\dfrac{17}{6}×\dfrac{3}{2}=\\[2em]
\dfrac{2}{3}×\dfrac{9}{2}=\qquad
\dfrac{6}{5}×\dfrac{14}{2}=\qquad
\dfrac{16}{7}×\dfrac{28}{4}=\\[2em]
\dfrac{29}{2}×6=\qquad
\dfrac{1}{2}×7=\qquad
\dfrac{1}{4}×9=\\[2em]
\dfrac{4}{3}×9=\qquad
\dfrac{9}{4}×11=\qquad
\dfrac{3}{15}×\dfrac{2}{9}=\\[2em]
\dfrac{5}{7}×\dfrac{7}{5}=\qquad
\dfrac{1}{23}×\dfrac{9}{2}=\qquad
\dfrac{24}{4}×\dfrac{1}{6}=$
